Try a harder problem for timeout test

Test/prover/z3-hard-timeout.bpl
@@ -1,9 +1,11 @@
 // RUN: %boogie /proverOpt:C:"-T:1" /proverOpt:BATCH_MODE=true /trace "%s" > "%t"
 // RUN: %OutputCheck --file-to-check "%t" "%s"
-// CHECK-L: z3-hard-timeout.bpl(8,3): Error: This assertion might not hold.
+// CHECK-L: z3-hard-timeout.bpl(10,3): Error: This assertion might not hold.
 
-procedure SquareRoot2NotRational(p: int, q: int)
-{
-  assume p > 0 && q > 0;
-  assert (p * p) !=  2 * (q * q);
+function {:bvbuiltin "bvmul"}  BV256_MULT(x:bv256, y:bv256) returns  (bv256);
+function {:bvbuiltin "bvugt"}  BV256_UGT(x:bv256, y:bv256)   returns  (bool);
+procedure FactorPrime(a: bv256, b: bv256) {
+  assume BV256_UGT(a, 1bv256);
+  assume BV256_UGT(b, 1bv256);
+  assert BV256_MULT(a,b) != 6189700192562690137449562111bv256;
 }
